>[!note] Variance
>For a random variable with expectation $\mathbb{E}[X]=\upmu$,
>$$Var(X)=\mathbb{E}[(X-\upmu)^2]=\mathbb{E}[X^2] - \upmu^2.$$
>Then the square root $\sigma(X)=\sqrt{Var(X)}$ is the standard deviation of $X$, and
>$Var(cX)=c^2Var(X).$
>
#### Proof.
We will now prove the steps to go from the middle to the RHS of the above equation. Firstly, we take $Var(X)=\mathbb{E}[(X-\upmu)^2]$ and $\mathbb{E}[X]=\upmu$. We proceed as follows:
$$
\begin{equation}
\begin{aligned}
Var(X) &= \mathbb{E}[(X-\upmu)^2] \\
&= \mathbb{E}[X^2-2\upmu X+\upmu^2] \\
&= \mathbb{E}[X^2]-2\upmu\mathbb{E}[X]+\upmu^2 \\
&= \mathbb{E}[X^2]-2\upmu \times \upmu + \upmu^2 \\
&= \mathbb{E}[X^2]-\upmu^2
\end{aligned}
\end{equation}
$$
We also need to prove the identity $Var(cX)=c^2Var(X)$. An important note here is that  [[3.1b Linearity of Expectation|linearity of expectation]] leads us to $\mathbb{E}[cX]=c\mathbb{E}[X]=c \upmu$ instead of just $\upmu$. Knowing this, we proceed as follows:
$$
\begin{equation}
\begin{aligned}
Var(cX) &=\mathbb{E}[(cX-c\upmu)^2] \\
&= \mathbb{E}[c^2(X-\upmu)^2] \\
&= c^2\mathbb{E}[(X-\upmu)^2] \\
&= c^2Var(X)
\end{aligned}
\end{equation}
$$

> [!example] 
> 