>[!note] Constant + MSE Solution
>The solution to the [[4.2b.1 Constant Model|constant model]] fitted with [[4.1b Squared Loss|L2 Loss]] is
>$$\hat{\theta}_0 = \bar{y}.$$
# Proof
First we differentiate MSE with respect to $\theta_0$:
$$\frac{d}{d \theta_0}MSE=\frac{-2}{n}\sum^{n}_{i=1}(y_i-\theta_0)$$
Then, we set $\frac{d}{d \theta_0}MSE=0$:
$$0 =\frac{-2}{n}\sum^{n}_{i=1}(y_i-\hat{\theta}_0) \iff \sum^{n}_{i=1}y_i=n \hat{\theta}_0$$
Therefore, we find that
$$\hat{\theta}_0=\frac{1}{n}\sum y_i=\bar{y}.$$
