>[!note] Constant + MAE Solution
>The solution to the [[4.2b.1 Constant Model|constant model]] fitted with [[4.1a Absolute Loss|L1 Loss]] is
>$$\hat{\theta}_0 = median(y).$$
# Proof
We cannot go straight to differentiation since absolute values are undefined at 0 (or when $y_i=\theta_0$). Therefore, we need to separate the loss function into piecewise cases:
$$
|y_i-\theta_0|=
\begin{cases}
y_i - \theta_0 & \text{if } \theta_0<y_i \\
\theta_0 - y_i & \text{if } \theta_0>y_i
\end{cases}
$$

Then we differentiate the loss function with respect to $\theta_0$:
$$\frac{d}{d \theta_0}|y_i-\theta_0|=
\begin{cases}
-1 & \text{if } \theta_0<y_i \\
1 & \text{if } \theta_0>y_i
\end{cases}
$$
We can summarize this piecewise case as
$$\frac{d}{d \theta_0}MAE=\frac{1}{n}\sum^{n}_{i=1}\frac{d}{d \theta_0}|y_i-\theta_0|=\frac{1}{n}\left[\sum^{}_{\theta_0<y_i}(-1)+\sum^{}_{\theta_0>y_i}(1)\right]$$

Then, we set $\frac{d}{d \theta_0}MAE=0$:
$$0=\frac{1}{n}\left[\sum^{}_{\theta_0<y_i}(-1)+\sum^{}_{\theta_0>y_i}(1)\right] \iff\sum^{}_{\theta_0<y_i}(1)=\sum^{}_{\theta_0>y_i}(1)$$
Which means that the amount of observations greater than $\theta_0$ must be equal to the amount of observations less than $\theta_0$, or, in other words,
$$\hat{\theta}_0 = median(y).$$
