>[!note] Sum of Independent Poisson Random Variables
>For two independent random variables $X$ and $Y$ with parameters $\uplambda$ and $\upmu$ respectively,
>$$X+Y \enspace \textasciitilde \enspace \text{Poisson}(\uplambda + \upmu).$$
#### Proof.
Since we are talking about [[2.3 Independent Random Variables|independent random variables]] of the [[4.6 Poisson Distribution|Poisson distribution]], we can proceed as follows:
$$
\begin{equation}
\begin{aligned}
\mathbb{P}[X+Y=k] &= \sum^{k}_{j=0}\mathbb{P}[X=j,Y=k-j] \\
&= \sum^{k}_{j=0}\mathbb{P}[X=j]\times \mathbb{P}[Y=k-j] \\
&= \sum^{k}_{j=0}\frac{\uplambda^{j}}{j!}e^{-\uplambda} \times \frac{\upmu^{k-j}}{(k-j)!}e^{-\upmu} \\
&= e^{-(\uplambda+\upmu)} \frac{1}{k!}\sum^{k}_{j=0}\frac{k!}{(k-j)!j!}\uplambda^j \upmu^{k-j} \\
&= e^{-(\uplambda+\upmu)} \frac{1}{k!}\binom{k}{j}\uplambda^j \upmu^{k-j} \\
&= \frac{(\uplambda+\upmu)^k}{k!}e^{-(\uplambda+\upmu)}
\end{aligned}
\end{equation}
$$
Where in line 6 the [[6.4 Binomial Theorem|binomial theorem]] is used.