>[!note] Consumption Function
>For $MU(c)=\frac{1}{c}$, consumption can be derived as
>$$c_1=\frac{1}{1+\beta}\left(y_1+\frac{y_2}{1+r}\right).$$
>Similarly, savings can be derived as
>$$s_1 = y_1 - c_1 = \frac{\beta}{1+\beta}y_1 - \frac{1}{1+\beta}\left(\frac{y_2}{1+r}\right).$$
>Implications of the consumption-savings framework include:
>1. Consumption Smoothing 
# Intuition
Using $MU(c)=\frac{1}{c}$ in the [[1.2 Maximizing Utility|tangency condition]], we get
$$c_2=\beta(1+r)c_1.$$
Then, replacing $c_2$ in the [[1.3 Intertemporal Budget Constraint|budget constraint]],
$$c_1+\frac{\beta(1+r)c_1}{1+r}=y_1+\frac{y_2}{1+r}$$
and we can see how we can solve for $c_1$.