---
{}
---
>[!note] Vector Addition
>The [[1.2d Vector Operations|operation]] for the sum of two vectors of the same size and in the same space (belonging to $\mathbb{R}^n$), $\vec{x}=\begin{bmatrix} x_1 & x_2 & \dots & x_n \end{bmatrix}^T$ and $\vec{y}=\begin{bmatrix} y_1 & y_2 & \dots & y_n \end{bmatrix}^T$ is
>$$\vec{x}+\vec{y}=\begin{bmatrix} x_1 + y_1 \\ x_2 + y_2 \\ \vdots \\ x_n + y_n \end{bmatrix}.$$

# Explanation
We can illustrate vector addition on the Cartesian plane. If we use the vectors $\vec{x}=\begin{bmatrix}2 \\ 2\end{bmatrix}$ and $\vec{y}=\begin{bmatrix}1 \\ 2\end{bmatrix}$, we can plot them on the x-y axis as
```tikz
\begin{document}
\begin{tikzpicture}[domain=0:4]
  \draw[<->] (-1,0)--(3,0) node[right]{$x$};
  \draw[<->] (0,-1)--(0,3) node[above]{$y$};
  \draw[->, thick, green](0,0)--(2,2) node[above]{$\vec{x}$};
  \draw[->, thick, red](0,0)--(1,2) node[above]{$\vec{y}$};
\end{tikzpicture}
\end{document}
```
We can think of vector addition in a multitude of ways, but it can be represented the same as a vector itself; you walk x steps over the x-axis, and y steps over the y-axis. Order doesn't matter, so $\vec{x}+\vec{y}=\vec{y}+\vec{x}=\begin{bmatrix}3 \\ 4\end{bmatrix}$,
```tikz
\begin{document}
\begin{tikzpicture}
  \draw[<->] (-1,0)--(4,0) node[right]{$x$};
  \draw[<->] (0,-1)--(0,4) node[above]{$y$};
  \draw[->, thick, green]( 1,2)--(3,4) node[above]{$\vec{x}$};
  \draw[->, thick, red] (0,0)--(1,2) node[above]{$\vec{y}$};
  \draw[->, thick, dashed, orange] (0,0)--(3,4) node[right, yshift=-60, xshift=-40]{$\vec{x}+\vec{y}$};
\end{tikzpicture}
\begin{tikzpicture}[domain=0:4]
  \draw[<->] (-1,0)--(4,0) node[right]{$x$};
  \draw[<->] (0,-1)--(0,4) node[above]{$y$};
  \draw[->, thick, green] (0,0)--(2,2) node[above]{$\vec{x}$};
  \draw[->, thick, red] (2,2)--(3,4) node[above]{$\vec{y}$};
  \draw[->, thick, dashed, orange] (0,0)--(3,4) node[left, yshift=-50, xshift=-40]{$\vec{x}+\vec{y}$};
\end{tikzpicture}
\end{document}
```
Vector subtraction is based on the same principle, with the crucial difference that the vector is reversed (flipped over x). However, note that $\vec{y}-\vec{x}=\begin{bmatrix}-1 \\ 0\end{bmatrix}$ is not the same as $\vec{x}-\vec{y}=\begin{bmatrix}1 \\ 0\end{bmatrix}$ (but it always is its negative!), unless $\vec{x}=\vec{y}$.

